Replace `Build_Class` with `Build_Trait`
And implement required traits in the rust example

examples/traits/traits_parms.rs
@@ -10,6 +10,10 @@ trait SomeTrait {
 
 struct SomeOtherType(u32);
 
+impl Foo for SomeOtherType {}
+impl Bar for SomeOtherType {}
+impl Tar for SomeOtherType {}
+
 impl SomeTrait for SomeOtherType {
     fn some_fn() {}
 }
