coq_translation/examples/traits/traits_parms.v
@@ -49,6 +49,27 @@ Module SomeOtherType.
 End SomeOtherType.
 Definition SomeOtherType := SomeOtherType.t.
 
+Module Impl_traits_parms_Foo_for_traits_parms_SomeOtherType.
+  Definition Self := traits_parms.SomeOtherType.
+  
+  Global Instance I : traits_parms.Foo.Trait Self :=
+    traits_parms.Foo.Build_Trait _.
+End Impl_traits_parms_Foo_for_traits_parms_SomeOtherType.
+
+Module Impl_traits_parms_Bar_for_traits_parms_SomeOtherType.
+  Definition Self := traits_parms.SomeOtherType.
+  
+  Global Instance I : traits_parms.Bar.Trait Self :=
+    traits_parms.Bar.Build_Trait _.
+End Impl_traits_parms_Bar_for_traits_parms_SomeOtherType.
+
+Module Impl_traits_parms_Tar_for_traits_parms_SomeOtherType.
+  Definition Self := traits_parms.SomeOtherType.
+  
+  Global Instance I : traits_parms.Tar.Trait Self :=
+    traits_parms.Tar.Build_Trait _.
+End Impl_traits_parms_Tar_for_traits_parms_SomeOtherType.
+
 Module Impl_traits_parms_SomeTrait_for_traits_parms_SomeOtherType.
   Definition Self := traits_parms.SomeOtherType.
   
